x86model/RockSalt/FastVerifier.v
@@ -20,7 +20,7 @@ Require Import Recognizer.
 Require Import Int32.
 Require Import VerifierDFA.
 
-Import X86_PARSER_ARG.
+Import ParserArg.X86_PARSER_ARG.
 Import X86_PARSER.
 (* Import X86_BASE_PARSER. *)
 
